src/coq/formula.v
@@ -13,8 +13,8 @@ Module Type Formulas.
   Definition Valuation : Type := Var -> Model .
 
   Parameter var_eq : Var -> Var -> bool .
-  Axiom var_eq_spec_true : forall x y, var_eq x y = true <-> x = y .
-  Axiom var_eq_spec_false : forall x y, var_eq x y = false <-> x <> y .
+  Axiom var_eq_true : forall x y, var_eq x y = true <-> x = y .
+  Axiom var_eq_false : forall x y, var_eq x y = false <-> x <> y .
   Axiom var_eq_refl : forall x, var_eq x x = true .
   
   (* FOL *)
@@ -76,6 +76,17 @@ Module Type Formulas.
   (* Free variables *)
   Parameter getFreeVars : MLFormula -> list Var .
 
+  Axiom freeVars_ExistsML :
+    forall phi x X,
+      In x (getFreeVars (ExistsML X phi)) <->
+      In x (getFreeVars phi) /\ ~ In x X .
+
+  Axiom freeVars_AndML :
+    forall phi phi' x,
+      In x (getFreeVars (AndML phi phi')) <->
+      In x (getFreeVars phi) \/ In x (getFreeVars phi').
+
+  
   (* Modify valuation on set *)
   Definition modify_val_on_var(rho rho' : Valuation) (x : Var) : Valuation :=
     fun z => if (var_eq x z) then rho' x else rho z .
@@ -89,20 +100,50 @@ Module Type Formulas.
   Lemma modify_in :
     forall V x rho rho',
       In x V -> (modify_val_on_set rho rho' V) x = rho' x.
-  Admitted.
+  Proof.
+    induction V; intros.
+    - contradiction.
+    - simpl in *.
+      destruct H as [H | H].
+      + subst a.
+        unfold modify_val_on_var.
+        rewrite var_eq_refl.
+        reflexivity.
+      + unfold modify_val_on_var.
+        case_eq (var_eq a x); intros H'.
+        * apply var_eq_true in H'.
+          subst a.
+          reflexivity.
+        * apply IHV; trivial.
+  Qed.
     
   
   Lemma modify_not_in :
-    forall x V rho rho',
+    forall V x rho rho',
       ~ In x V -> (modify_val_on_set rho rho' V) x = rho x.
-  Admitted.
+  Proof.
+    induction V; intros.
+    - simpl.
+      reflexivity.
+    - simpl in *.
+      apply not_or_and in H.
+      destruct H as (H & H').
+      unfold modify_val_on_var.
+      case_eq (var_eq a x); intros H''.
+      + apply var_eq_true in H''.
+        subst a.
+        contradict H.
+        reflexivity.
+      + apply IHV; trivial.
+  Qed.
 
   
   Lemma modify_Sat1 :
-    forall gamma rho rho' phi V,
+    forall phi V gamma rho rho',
       SatML gamma rho' phi ->
       incl (getFreeVars phi) V ->
       SatML gamma (modify_val_on_set rho rho' V) phi.
+  Proof.
   Admitted.
   
   Lemma modify_Sat2 :
@@ -113,191 +154,15 @@ Module Type Formulas.
   Admitted.
   
   
-  (* renaming stuff *)
-  Parameter rename_var : Var -> Var -> MLFormula -> MLFormula.
-
-  Axiom new_var_is_free :
-    forall x y phi,
-      In x (getFreeVars phi) ->
-      In y (getFreeVars (rename_var x y phi)) .
-
-  Axiom new_or_old :
-    forall x y z phi,
-      In z (getFreeVars (rename_var x y phi)) ->
-      z = y \/ (z <> y /\ In z (getFreeVars phi)) .
-  
-  
-  Fixpoint rename_var_set (X Y : list Var)
-           (phi : MLFormula) : MLFormula :=
-    match X, Y with
-      | x :: Xs, y :: Ys =>
-        rename_var x y (rename_var_set Xs Ys phi)
-(*        rename_var_set Xs Ys (rename_var x y phi) *)
-      | _, _ => phi
-    end.
-          
-  
-  Definition rename_val (rho : Valuation) (x y : Var) : Valuation :=
-    fun z => if (var_eq z y) then rho x else rho z .
-
-  Lemma rename_val_not_in :
-    forall z rho x y,
-      z <> x ->  rename_val rho x y z = rho z.
-  Admitted.
-  
-  
-  Lemma rename_sat :
-    forall gamma rho phi x y,
-      SatML gamma rho phi ->
-      ~ In y (getFreeVars phi) ->
-      SatML gamma (rename_val rho x y) (rename_var x y phi) .
-  Admitted.
-
-  Fixpoint rename_val_set (rho : Valuation) (X Y : list Var) : Valuation :=
-    match X, Y with 
-      | x :: Xs, y :: Ys =>
-        rename_val_set (rename_val rho x y) Xs Ys 
-      | _, _ => rho
-    end.
-
-  Lemma rename_sat_set :
-    forall gamma rho phi X Y,
-      SatML gamma rho phi ->
-      (forall y, In y Y -> ~ In y (getFreeVars phi)) ->
-      SatML gamma (rename_val_set rho X Y) (rename_var_set X Y phi).
-  Admitted.
-
-  Lemma rename_val_set_not_in :
-    forall v rho X Y,
-      ~ In v X -> rename_val_set rho X Y v = rho v.
-  Admitted.
-  
-  
-
-  
-(*
-  Lemma rename_sat_Set :
-    forall gamma rho phi X Y,
-      SatML gamma rho phi <->
-      SatML gamma rho (rename_vars X Y phi) .
-  Proof.
-    intros gamma rho phi X Y.
-    split; intros H.
-    - induction X.
-      + simpl; trivial.
-      + simpl.
-  Admitted.
-*)  
-
-  Axiom rename_And :
-    forall phi phi' X Y,
-      rename_var_set X Y (AndML phi phi') =
-      (AndML (rename_var_set X Y phi) (rename_var_set X Y phi')).
-
-  Axiom rename_Not :
-    forall phi X Y,
-      rename_var_set X Y (NotML phi) =
-      (NotML (rename_var_set X Y phi)).
-
-  
-  Parameter generate_var_not_in_set : list Var -> Var .
-  Axiom new_var_not_in_set :
-    forall X,
-       ~ In (generate_var_not_in_set X) X.
-
-  Fixpoint generate_vars (n : nat) (X : list Var) : list Var :=
-    match n with
-      | 0 => nil
-      | S n' => let new_x := generate_var_not_in_set X in
-                new_x :: generate_vars n' (new_x :: X)
-    end.
-
-  Lemma generate_vars_exact_n :
-    forall n X,
-      n = length (generate_vars n X) .
-  Proof.
-    induction n; simpl; trivial.
-    intros X.
-    apply eq_S.
-    apply IHn.
-  Qed.
-
-    
-
-
-  Lemma replace_all :
-    forall phi Y X y,
-      incl (getFreeVars phi) X ->
-      length X = length Y ->
-      (In y (getFreeVars (rename_var_set X Y phi)) <-> In y Y).
-  Proof.
-  Admitted.      
-    
-
-
-      
-      
-  
-  Lemma generated_vars_not_in_set :
-    forall n X y,
-      In y (generate_vars n X) ->
-      ~ In y X.
-  Proof.
-    induction n; intros.
-    - simpl in H.
-      contradict H.
-    - simpl in H.
-      destruct H as [H | H].
-      + subst y.
-        apply new_var_not_in_set.
-      + apply IHn in H.
-        unfold not in *.
-        intros.
-        apply H.
-        simpl.
-        right.
-        trivial.
-  Qed.
-
-  Lemma generated_vars_not_in :
-    forall n x X Y,
-      In x X ->
-      incl X Y ->
-      ~ In x (generate_vars n Y) .
-  Proof.
-    induction n; intros.
-    - simpl.
-      unfold not.
-      intros.
-      trivial.
-    - simpl.
-      apply and_not_or.
-      split.
-      + assert (H1 : ~ In (generate_var_not_in_set Y) Y).
-        * apply new_var_not_in_set.
-        * unfold not.
-          intros.
-          subst x.
-          unfold incl in H0.
-          apply H0 in H.
-          contradict H1.
-          trivial.
-      + apply IHn with (X := X); trivial.
-        unfold incl.
-        intros a Ha.
-        simpl.
-        right.
-        unfold incl in H0.
-        apply H0 in Ha; trivial.
-  Qed.
-
-
-
   
   (* encoding: ML -> FOL *)
   (* Parameter encoding : MLFormula -> FOLFormula . *)
   Parameter encoding : MLFormula -> MLFormula .
 
+  Axiom freeVars_encoding :
+    forall phi x,
+      In x (getFreeVars (encoding phi)) <-> In x (getFreeVars phi) .
+    
   (* encoding properties *)
   (* 
     The following proposition, looks cleaner when 
@@ -311,17 +176,5 @@ Module Type Formulas.
     forall gamma' phi rho,
       SatML gamma' rho (encoding phi) <->
       exists gamma, SatML gamma rho phi.
-
-  
-  Axiom enc_sat :
-    forall gamma rho phi,
-      SatML gamma rho (encoding phi) <->
-      SatML gamma rho phi.
-  
-
-  Axiom rename_encoding :
-    forall phi X Y,
-      rename_var_set X Y (encoding phi) =
-      (encoding (rename_var_set X Y phi)).
   
 End Formulas.
